

7/10/25-

Consider the (LH) system-

$$\dot{x}(t) = A(t)x(t)$$

Suppose f_1, \dots, f_n be solns. of (LH). Consider

$$U(t) = [f_1(t), \dots, f_n(t)]$$

then $U(t)$ satisfies

$$U'(t) = A(t)U(t)$$

$$f_j'(t) = A(t)f_j(t)$$

Consider $(A(t)U(t))_{i,j} = \sum_{k=1}^n (A(t))_{i,k} (U(t))_{k,j}$

$$= \sum_{k=1}^n (A(t))_{i,k} f_{j,k}(t)$$

Here $f_j(t) = (f_{j,1}(t), \dots, f_{j,n}(t))$

$$\Rightarrow (A(t)f_j(t))_{i,1} = (f_j(t))_{i,1} = f_{j,i}(t) = (U(t))_{i,j}$$

$U(t)$ is a solution matrix.

• Note that the principal soln. matrix at a point t_0 , $\Phi(\cdot, t_0)$ is a solution matrix.

Defⁿ:- Given homogeneous system,

$$x'(t) = A(t)x(t)$$

$A: I \xrightarrow{\text{cont.}} M_n(\mathbb{R})$. A matrix valued fncⁿ $\psi: I \rightarrow M_n(\mathbb{R})$ is called

a fundamental soln. matrix if $\psi(t)$ satisfies the following two conditions

① $\psi'(t) = A(t)\psi(t) \quad \forall t \in I$

② the columns of ψ are linearly independent in $C(I, \mathbb{R}^n)$.

Note the principal soln. matrix is a fundamental matrix.

THEOREM: A necessary & sufficient condition that a solution matrix $\psi: I \rightarrow M_n(\mathbb{R})$

be a fundamental soln. matrix is that $\det(\psi(t)) \neq 0$ for some $t \in I$.

PROOF: First suppose $\psi: I \rightarrow M_n(\mathbb{R})$ is a fundamental soln. matrix.

$$\psi(t) = [\psi_1(t) \dots \psi_n(t)] \quad t \in I$$

Claim: Fix $t_0 \in I$ then the vector $(\psi_1(t_0), \dots, \psi_n(t_0))$ are lin. ind.

Suppose not. $\sum_{i=1}^n c_i \psi_i(t_0) = 0$, where not all c_i 's are zero.

Let $\phi = \sum_{i=1}^n c_i \psi_i$, then ϕ is also a soln. of (LH).

$$\phi(t_0) = \left(\sum_{i=1}^n c_i \psi_i \right) t_0 = \sum_{i=1}^n c_i \psi_i(t_0)$$

$$\Rightarrow \phi \equiv 0$$

$$\sum_{i=1}^n c_i \psi_i \equiv 0 \Rightarrow \underbrace{\{\psi_1, \dots, \psi_n\}}_X \text{ are lin. dep. which is a contradicⁿ.$$

Now suppose $\psi'(t) = A(t)\psi(t)$

Suppose for some $t_0 \in I$, $\det(\psi(t_0)) \neq 0$

Claim: (ψ_1, \dots, ψ_n) are lin. ind.

Suppose not. Then $\sum_{i=1}^n c_i \psi_i \equiv 0$, where not all c_i 's are zero.

$$\Rightarrow \sum_{i=1}^n c_i \psi_i(t_0) = 0 \quad \text{Not all } c_i \text{'s are zero.}$$

$$\psi(t_0)C = 0$$

$$C = \begin{pmatrix} c_1 \\ \vdots \\ c_n \end{pmatrix}$$

$$\Rightarrow \det(\psi(t_0)) = 0 \quad (\text{Contradiction})$$

—X—

$U(t) \leftarrow$ Solution matrix

$$W(t) = \det(U(t)) \quad t \in I$$

↖ Wronski deter.

If for some t_0 , $W(t_0) \neq 0$ then for any other t
 $W(t) \neq 0$

Exercise: $U(t) \leftarrow$ solution matrix

① $U(t)C$, $C \in M_n(\mathbb{R})$ is a soln. matrix.

② ψ_1, ψ_2 are two FSM then for any $t_0 \in I$

$$\psi_1(t)(\psi_1(t_0))^{-1} = \psi_2(t)(\psi_2(t_0))^{-1} = \Phi(t, t_0)$$

$$\dot{x}(t) = A(t)x(t) + \phi(t) \quad \text{--- ①}$$

ϕ_1, ϕ_2 then $\phi_1 - \phi_2$ is a solution of
 $\dot{x}(t) = A(t)x(t)$

This implies that if we know a particular solution of ①, ϕ_0 then all other solns. are given by $\phi_0 +$ soln. set of (LH)

$$\begin{aligned} & \phi_0 + \psi \\ \dot{x}(t) &= A(t)x(t) + \phi(t) \\ x(t_0) &= x_0 \end{aligned}$$

Suppose the soln. to be of the form

$$\phi(t) = \Phi(t, t_0)C(t)$$

13/10/2025

$$\dot{x}(t) = A(t)x(t) \quad x(t_0) = x_0$$

Soln. is given by $x(t) = \Phi(t, t_0)x_0$

Recall $\Phi(\cdot, t_0)$ is the principal soln. matrix.

$$(1) \Phi'(t, t_0) = A(t)\Phi(t, t_0)$$

$$(2) \Phi(t_0, t_0) = I_n$$

Inhomogeneous System

$$\dot{x}(t) = A(t)x(t) + g(t) \quad (\text{ILS})$$

$$A: I \xrightarrow{\text{cont.}} M_n(\mathbb{R})$$

$$g: I \xrightarrow{\text{cont.}} \mathbb{R}^n$$

Let ϕ_1, ϕ_2 be two soln. of (ILS). Then $\phi_1 - \phi_2$ is a soln. of (LH)

Hence, if we know a particular soln. ϕ of (ILS) then any other soln. is of the type $\psi + \phi$ where ψ is a soln. of (LH).

2. Consider (ILS) with the initial condition $x(t_0) = x_0$.

The idea is to guess that the soln. is of the form

$$\phi(t) = \Phi(t, t_0)c(t)$$

Observe that $\phi(t_0) = x_0 = c(t_0)$

$$\phi'(t) = \Phi'(t, t_0)c(t) + \Phi(t, t_0)c'(t)$$

$$= A(t)\Phi(t, t_0)c(t) + \Phi(t, t_0)c'(t)$$

$$= A(t)\phi(t) + \Phi(t, t_0)c'(t)$$

$$= A(t)\phi(t) + g(t) \quad [\text{By assumption}]$$

$$\begin{aligned}\Phi(t, t_0) c'(t) &= g(t) \\ \Rightarrow c'(t) &= \Phi(t, t_0)^{-1} g(t) = \Phi(t_0, t) g(t) \\ \Rightarrow c(t) - c(t_0) &= \int_{t_0}^t \Phi(t_0, s) g(s) ds\end{aligned}$$

$$c(t) = x_0 + \int_{t_0}^t \Phi(t_0, s) g(s) ds$$

Our soln. :- $\varphi(t) = \Phi(t, t_0) x_0 + \Phi(t, t_0) \int_{t_0}^t \Phi(t_0, s) g(s) ds$

$$\varphi(t) = \Phi(t, t_0) x_0 + \int_{t_0}^t \Phi(t, s) g(s) ds$$

1-d case: $x'(t) = a(t)x(t) + b(t)$

$$\begin{aligned}\Phi'(t, t_0) &= a(t) \Phi(t, t_0) \\ \Phi(t_0, t_0) &= 1 \\ \Phi(t, t_0) &= \exp\left(\int_{t_0}^t a(s) ds\right)\end{aligned}$$

Linear Differential Eqns. of order n:

HOMOGENEOUS CASE:

Consider a_0, a_1, \dots, a_n , cont. fncⁿs on I , assume $a_0(t) \neq 0$ for any $t \in I$. Consider the differential operator.

$$L_n = a_0(t) \frac{d^n}{dt^n} + a_1(t) \frac{d^{n-1}}{dt^{n-1}} + \dots + a_n(t)$$

acts on all fncⁿ on I that are at least n times differentiable.

$$L_n(g) = a_0(t) g^{(n)}(t) + a_1(t) g^{(n-1)}(t) + \dots + a_{n-1}(t) g^{(1)}(t) + a_n(t) g(t)$$

The linear diff. eqn. of order n is the eqn.

$$L_n x = 0 \Leftrightarrow a_0(t) x^{(n)}(t) + a_1(t) x^{(n-1)}(t) + \dots + a_{n-1}(t) x^{(1)}(t) + a_n(t) x(t) = 0$$

$$x^{(n)}(t) + \frac{a_1(t)}{a_0(t)} x^{(n-1)}(t) + \dots + \frac{a_{n-1}(t)}{a_0(t)} x^{(1)}(t) + \frac{a_n(t)}{a_0(t)} x(t) = 0 \quad \text{--- ①}$$

* Introduce $(y_1, y_2, \dots, y_n) = (x(t), x^{(1)}(t), \dots, x^{(n-1)}(t))$

$$\begin{aligned}y_1 &= y_2 \\ y_2' &= y_3 \\ &\vdots \\ y_{n-1}' &= y_n \\ y_n' &= -\frac{a_1(t)}{a_0(t)} y_{n-1} - \frac{a_2(t)}{a_0(t)} y_{n-2} - \dots - \frac{a_{n-1}(t)}{a_0(t)} y_1\end{aligned}$$

$$y'(t) = A(t) y(t) \quad \text{--- ②} \quad A(t) = \begin{pmatrix} 0 & 1 & 0 & 0 & \dots & 0 \\ 0 & 0 & 1 & 0 & \dots & 0 \\ \vdots & \vdots & \vdots & \vdots & \ddots & \vdots \\ 0 & 0 & 0 & \dots & 0 & 1 \\ -\frac{a_{n-1}(t)}{a_0(t)} & -\frac{a_{n-2}(t)}{a_0(t)} & \dots & -\frac{a_2(t)}{a_0(t)} & -\frac{a_1(t)}{a_0(t)} & 0 \end{pmatrix} \begin{pmatrix} y_1 \\ y_2 \\ \vdots \\ y_{n-1} \\ y_n \end{pmatrix}$$

1) Observe that if φ is a soln. of
 ① i.e. $L_n \varphi = 0$.
 Then $(\varphi, \varphi', \dots, \varphi^{(n-1)})$ is a soln. of ②

2) Suppose $\varphi = \begin{pmatrix} \varphi_1 \\ \vdots \\ \varphi_n \end{pmatrix}$ is a soln. of ②. Then

$$\begin{aligned} \varphi_2 &= \varphi_1' \\ \varphi_3 &= \varphi_2' = \varphi_1'' \\ &\vdots \\ \varphi_{n-1} &= \varphi_1^{(n-2)} \\ \varphi_n &= \varphi_1^{(n-1)} \quad \& \quad \varphi_1 \text{ satisfies} \\ L_n \varphi_1 &= 0 \end{aligned}$$

14/10/2025

$$\begin{aligned} L_n x &= 0 \quad \text{--- ①} \\ L_n &= a_0 \frac{d^n}{dt^n} + a_1 \frac{d^{n-1}}{dt^{n-1}} + \dots + a_{n-1} \frac{d}{dt} + a_n \\ L_n x &\equiv 0 \iff y' = A(t)y \quad \text{--- ②} \\ \varphi &\iff (\varphi, \varphi', \dots, \varphi^{(n-1)}) \end{aligned}$$

$$A(t) = \begin{pmatrix} 0 & 1 & 0 & 0 & \dots & 0 \\ 0 & 0 & 1 & 0 & \dots & 0 \\ & & \vdots & & & \\ 0 & 0 & 0 & 0 & \dots & 1 \\ \frac{-a_n(t)}{a_0(t)} & \frac{-a_{n-1}(t)}{a_0(t)} & \dots & \dots & \dots & \frac{-a_1(t)}{a_0(t)} \end{pmatrix}$$

1) Notice that given $t_0 \in I$ & $y \in \mathbb{R}^n$, we know that
 there is a unique soln. φ of $y' = A(t)y$. WHY?
 If we write $\varphi = (\varphi_1, \dots, \varphi_n)$ then
 $\varphi(t_0) = x_0 = (x_{01}, x_{02}, \dots, x_{0n})$

$$\begin{aligned} \varphi(t_0) &= (\varphi_1(t_0), \varphi_1'(t_0), \dots, \varphi_1^{(n-1)}(t_0)) \\ &= (x_{01}, x_{02}, \dots, x_{0n}) \\ L_n \varphi_1 &= 0 \end{aligned}$$

2) Now let $\varphi_1, \dots, \varphi_n$ be soln. of
 $L_n x = 0$

Consider the matrix

$$\Phi = \begin{pmatrix} \varphi_1 & \varphi_2 & \dots & \varphi_n \\ \varphi_1^{(1)} & \varphi_2^{(1)} & \dots & \varphi_n^{(1)} \\ \vdots & \vdots & & \vdots \\ \varphi_1^{(n-1)} & \varphi_2^{(n-1)} & \dots & \varphi_n^{(n-1)} \end{pmatrix} = [\Phi_1, \dots, \Phi_n]$$

This is a soln. matrix for the linear system
 $y' = A(t)y$

The determinant of the soln. matrix is called the Wronskian associated to ϕ_1, \dots, ϕ_n denoted by

$$W(\phi_1, \dots, \phi_n)(t) = |\Phi|$$

LEMMA: $x'(t) = A(t)x(t)$. Let $U(t)$ be a soln. matrix i.e.

$$U'(t) = A(t)U(t). \text{ Then}$$

$$|U(t)| = |U(t_0)| \exp\left(\int_{t_0}^t \text{trace}(A(s)) ds\right) \leftarrow \text{Abel's Identity}$$

$$|U(t)|' = \text{trace}(A(t)) |U(t)|$$

THEOREM: Every soln. of $L_n x = 0$ is a linear combination of any n -linearly independent solutions. Given ϕ_1, \dots, ϕ_n solution of $L_n x = 0$ they are lin. ind. iff
 $W(\phi_1, \dots, \phi_n) \neq 0$ on I

PROOF: Soln. set $L_n x = 0 \xrightarrow[\text{onto}]{\text{one-one}} \text{Soln. set of } y' = A(t)y(t)$
 $L: \phi \mapsto (\phi, \phi^{(1)}, \dots, \phi^{(n-1)})$
 $L(\phi) = (\phi, \phi^{(1)}, \dots, \phi^{(n-1)})$ is a vector space isomorphism i.e.

① L is one-one and onto.

$$\textcircled{2} L(\alpha\phi + \beta\psi) = \alpha L(\phi) + \beta L(\psi)$$

$\alpha, \beta \in \mathbb{R}, \phi, \psi$ solns. of $L_n x = 0$

The soln. space of $L_n x = 0$ is n -dim.

Suppose ϕ_1, \dots, ϕ_n are lin. ind. solns. of $L_n x = 0$. Then the matrix Φ is a fundamental soln. matrix.

$$W(\phi_1, \dots, \phi_n)(t) \neq 0 \quad \forall t \in I$$

THEOREM: Let ϕ_1, \dots, ϕ_n be functions on I such that $W(\phi_1, \dots, \phi_n)(t) \neq 0$ on I .

Then there exists a unique DE of order n^* for which these functions form a fundamental set, namely:

$$\frac{W(x, \phi_1, \dots, \phi_n)}{W(\phi_1, \dots, \phi_n)} = 0$$

DEF.: A set of n lin. ind. solns. of $L_n x = 0$ is called a fundamental set for $L_n x = 0$.

* where coefficients of higher order is 1.

16/10/2025

EXAMPLE: Consider fnc's

$$f_1(t) = t, f_2(t) = te^t$$

$I = (a, b)$ not containing 0 then

$$W(f_1, f_2)(t) = \begin{vmatrix} f_1 & f_2 \\ f_1' & f_2' \end{vmatrix} = \begin{vmatrix} t & te^t \\ 1 & te^t + e^t \end{vmatrix} = t^2 e^t$$

$$W(f_1, f_2)(t) \neq 0 \text{ for any } t \in (a, b)$$

$$\Rightarrow \frac{W(x, f_1, f_2)}{W(f_1, f_2)} = 0$$

x	t	te^t	$= 0$
\dot{x}	1	$te^t + e^t$	
\ddot{x}	0	$te^t + 2e^t$	

$$x(te^t + 2e^t) - \dot{x}(t^2e^t + 2te^t) + \ddot{x}(t^2e^t) = 0$$

Reduction of order of a DE :-

$$L_n x = 0$$

$$a_0(t)x^{(n)} + a_1(t)x^{(n-1)} + \dots + a_{n-1}(t)x^{(1)} + a_n(t)x = 0 \text{ --- ①}$$

Say, $f(t)$ is a soln.

$$\text{We write } x(t) = f(t)y(t)$$

$$\frac{dx}{dt} = f'(t)y(t) + f(t)y'(t)$$

$$\frac{d^n x}{dt^n} = f^{(n)}(t)y(t) + C_1^n f^{(n-1)}(t)y'(t) + \dots + C_{n-1}^n f'(t)y^{(n-1)}(t) + f(t)y^{(n)}(t)$$

$$a_0(t)(f(t)y^{(n)}(t) + C_1^n f'(t)y^{(n-1)} + \dots + f^{(n)}(t)y^{(1)}) + a_1(t)(f(t)y^{(n-1)}(t) + C_1^{n-1} f^{(1)}(t)y^{(n-2)}(t) + \dots + f^{(n-1)}(t)y(t)) + \dots + a_n(t)f(t)y(t) = 0$$

$$\Leftrightarrow a_0(t)f(t)y^{(n)} + (na_0(t)f^{(1)}(t) + (n-1)a_1(t)f(t))y^{(n-1)} + \dots + y(t)(a_0(t)f^{(n)}(t) + a_1(t)f^{(n-1)}(t) + \dots + a_n(t)f(t)) = 0 \text{ --- ②}$$

② reduces to

$$A_0(t)y^{(n)}(t) + A_1(t)y^{(n-1)}(t) + \dots + A_{n-1}(t)y^{(1)}(t) = 0 \text{ --- ③}$$

$$\text{Put } w = y'(t)$$

$$A_0(t)w^{(n-1)}(t) + A_1(t)w^{(n-2)}(t) + \dots + A_{n-1}(t)w(t) = 0 \text{ --- ④}$$

\Rightarrow Now suppose w_1, \dots, w_{n-1} is a known fundamental set of solutions for ④. Then $v_j(t) = \int w_j(t) dt, j=1, \dots, n-1$

& $v_n \equiv 1$ is a fundamental set of solutions for ③

$$\Leftrightarrow \begin{vmatrix} 1 & v_1 & v_2 & \dots & v_{n-1} \\ 0 & w_1^{(1)} & w_2^{(1)} & \dots & w_{n-1}^{(1)} \\ 0 & w_1^{(2)} & w_2^{(2)} & \dots & w_{n-1}^{(2)} \\ \vdots & \vdots & \vdots & \ddots & \vdots \\ 0 & w_1^{(n-1)} & w_2^{(n-1)} & \dots & w_{n-1}^{(n-1)} \end{vmatrix}$$

notice non-zero as $w_1, \dots, w_{n-1} \in I$

Finally for fundamental set of ①, multiply by $f(t)$ by (*)

Inhomogeneous

$$\Rightarrow L_n(x) = g(t) \quad x(t_0) = x_0 = (x(t_0), x'(t_0), \dots, x^{(n-1)}(t_0))$$

$$\Leftrightarrow x^{(n)}(t) + \frac{a_1(t)}{a_0(t)} x^{(n-1)}(t) + \dots + \frac{a_n(t)}{a_0(t)} x = \frac{g(t)}{a_0(t)}$$

$$\Leftrightarrow y'(t) = A(t)y(t) + \tilde{g}(t) \quad (y_1, \dots, y_n) = (x, x', \dots, x^{(n-1)})$$

$$\tilde{g}(t) = \begin{pmatrix} 0 \\ \vdots \\ 0 \\ \frac{g(t)}{a_0(t)} \end{pmatrix}$$

$$y(t_0) = x_0$$

$$(x(t_0), x'(t_0), \dots, x^{(n-1)}(t_0)) = x_0$$

The solution is given by

$$y(t) = \Phi(t, t_0)x_0 + \int_{t_0}^t \Phi(t, s)\tilde{g}(s)ds$$

where $\Phi(t, t_0)$ is the principal solution matrix.

$$\Phi'(t, t_0) = A(t)\Phi(t, t_0) \text{ and } \Phi(t_0, t_0) = I$$

$\varphi_j(t, t_0)$ is the solution of $L_n x = 0$ s.t.

$$(\varphi_j(t_0, t_0), \varphi_j^{(1)}(t_0, t_0), \dots, \varphi_j^{(n-1)}(t_0, t_0)) = e_j$$

21/10/2025

Class

Cancelled

24/10/2025

Order n differential equation

$$L_n = a_0(t) \frac{d^n}{dt^n} + a_1(t) \frac{d^{n-1}}{dt^{n-1}} + \dots + a_{n-1}(t) \frac{d}{dt} + a_n(t)$$

$$L_n x = g(t)$$

a_0, a_1, \dots, a_n are cts. fncⁿ on $I \subset \mathbb{R}$

HOMOGENEOUS CASE

$$L_n x = 0 \Leftrightarrow y'(t) = A(t)y(t)$$

INHOMOGENEOUS CASE

$$a_0(t) \frac{d^n x}{dt^n} + a_1(t) \frac{d^{n-1} x}{dt^{n-1}} + \dots + a_{n-1}(t) \frac{dx}{dt} + a_n(t) x(t) = g(t) \quad (*)$$

By considering the change of variable

$$y = (y_1, \dots, y_n) = (x, x', \dots, x^{(n-1)})$$

The associated linear system is given by

$$y'(t) = \begin{pmatrix} y_1' \\ \vdots \\ y_n' \end{pmatrix} = \begin{pmatrix} 0 & 1 & 0 & \dots & 0 \\ 0 & 0 & 1 & \dots & 0 \\ \vdots & \vdots & \vdots & \ddots & \vdots \\ 0 & 0 & 0 & \dots & 1 \\ -\frac{a_1}{a_0} & -\frac{a_2}{a_0} & \dots & -\frac{a_{n-1}}{a_0} & -\frac{a_n}{a_0} \end{pmatrix} \begin{pmatrix} y_1 \\ \vdots \\ y_n \end{pmatrix} + \begin{pmatrix} \tilde{g}(t) \\ 0 \\ \vdots \\ 0 \\ \frac{g(t)}{a_0(t)} \end{pmatrix}$$

This linear system has a unique soln., given $y(t_0) = y_0 \in \mathbb{R}^n$
 \Rightarrow This implies that given $t_0 \in I, y_0 \in \mathbb{R}^n, \exists$ unique soln. with
 $(x(t_0), x'(t_0), \dots, x^{(n-1)}(t_0)) = y_0$

The unique soln. of (***) is given by

$$y(t) = \underbrace{\Phi(t, t_0)}_{\text{Principal soln. matrix}} y_0 + \int_{t_0}^t \Phi(t, s) \tilde{g}(s) ds$$

Principal soln. matrix

First coordinate of ① given by

$$x(t) = \sum_{j=1}^n \Phi_{1j}(t, t_0) y_{0,j} + \int_{t_0}^t \Phi_{1n}(t, s) \frac{g(s)}{a_0(s)} ds$$

$$\Phi(t, s) = [\Phi_1(t, s) \dots \dots \Phi_n(t, s)]$$

$$\Phi_1'(t, s) = A(t) \Phi_1(t, s)$$

$$\Phi_1(s, s) = (1, 0, \dots, 0)$$

$$(\Phi_{ij}(t_0, t_0), \Phi_{ij}'(t_0, t_0), \dots, \Phi_{ij}^{(n-1)}(t_0, t_0)) = (0, \dots, 1, \dots, 0)$$

Linear Equations of order n with constant coefficients:-

$$x^{(n)} + a_1 x^{(n-1)} + \dots + a_n x = g(t)$$

Here a_1, \dots, a_n are constants

HOMOGENEOUS CASE

$$x^{(n)} + a_1 x^{(n-1)} + \dots + a_n x = 0 \text{ --- ①}$$

$$y' = Ay \text{ Associated linear system}$$

LEMMA: The characteristic polynomial of matrix A is given by:
 $f(\lambda) = \lambda^n + a_1 \lambda^{n-1} + \dots + a_n$

THEOREM:

Consider ①. Let $\lambda_1, \dots, \lambda_s$ be distinct eigenvalues of matrix A. Let m_i be the multiplicity of λ_i as a zero of $f(\lambda)$. Then the set of functions $t^k e^{\pm \lambda_i t}$, $k=0, \dots, m_i-1$ form a fundamental set of solns.

PROOF: $L_n(e^{\pm \lambda t}) = f(\lambda) e^{\pm \lambda t} \text{ --- ①}$
 $L_n(t^k e^{\pm \lambda t}) = L_n\left(\frac{\partial^k}{\partial \lambda^k} e^{\pm \lambda t}\right)$

$$= \frac{\partial^k}{\partial \lambda^k} (L_n(e^{\pm \lambda t})) = \frac{\partial^k}{\partial \lambda^k} (f(\lambda) e^{\pm \lambda t})$$

$$= \left(f^{(k)}(\lambda) + k f^{(k-1)}(\lambda) t + \frac{k(k-1)}{2} f^{(k-2)}(\lambda) t^2 \right. \\ \left. + \dots + f(\lambda) t^k \right) e^{\pm \lambda t} \text{ --- ②}$$

27/10/2025

Ordinary differential equation of order n with constant coefficients

$$L_n x = x^{(n)} + a_1 x^{(n-1)} + \dots + a_n x = 0$$

$$f(\lambda) = \lambda^n + a_1 \lambda^{n-1} + \dots + a_n$$

$$L_n = \frac{d^n}{dt^n} + a_1 \frac{d^{n-1}}{dt^{n-1}} + \dots + a_n$$

THEOREM: Let $\lambda_1, \dots, \lambda_s$ be distinct zeros of the polynomial $f(\lambda)$. Also let m_i be the multiplicity of λ_i as a zero of f .

$$(f(\lambda) = (\lambda - \lambda_i)^{m_i} g(\lambda))$$

Then $t^k e^{\lambda_i t}$, $k=0, \dots, m_i-1$ are fundamental solutions of ①.

FACT: λ_i has multiplicity m_i if the derivatives of f at λ_i vanish up to order m_i-1 .

PROOF: $\frac{d^k}{dt^k} (e^{\lambda t}) = \lambda^k e^{\lambda t}$

$$L_n (e^{\lambda t}) = f(\lambda) e^{\lambda t} \quad \text{--- ①}$$

$$L_n (t^k e^{\lambda t}) = L_n \left(\frac{\partial^k}{\partial \lambda^k} e^{\lambda t} \right) = \frac{\partial^k}{\partial \lambda^k} L_n (e^{\lambda t}) = \frac{\partial^k}{\partial \lambda^k} (f(\lambda) e^{\lambda t})$$

Periodic Linear Systems :-

$$\begin{aligned} \dot{x}(t) &= A(t)x(t) \\ A(t+\omega) &= A(t) \quad \forall t \text{ \& } \omega > 0 \end{aligned}$$

$$\frac{d^2 \theta}{dt^2} = -\frac{g}{L} \sin \theta$$

EXAMPLE: $\dot{x} = \sin^2 t x$
 $A(t) = \sin^2 t$
 $A(t+\pi) = A(t)$

$$\begin{aligned} x(t) &= c \exp\left(\frac{t}{2}\right) \exp\left(-\frac{\sin 2t}{4}\right) \\ c &\neq 0 \\ \dot{x} &= \sin t x(t) \end{aligned}$$

THEOREM (FLOQUET):- Consider the linear system

$$\dot{x}(t) = A(t)x(t) \quad \text{--- ①}$$

where $A: \mathbb{R} \rightarrow M_n(\mathbb{R})$ continuous with the least positive period ω , i.e.,
 $A(t) = A(t+\omega) \quad \forall t \in \mathbb{R}$.

Let ψ be a fundamental solution matrix of ① then

$$\psi_\omega(t) = \psi(\omega+t)$$

is a fundamental solution matrix. Furthermore,

$$\psi(t) = P(t) e^{Bt}$$

where $P: \mathbb{I} \rightarrow M_n(\mathbb{R})$ is a continuously differentiable periodic function with period ω and B is a complex matrix (constant)

THEOREM: Let C be a nonsingular matrix. Then $\exists B \in M_n(\mathbb{C})$ s.t.
 $e^B = C$

PROOF $n=2$

Case 1: Say, C diagonalisable; $J = \begin{pmatrix} \mu_1 & 0 \\ 0 & \mu_2 \end{pmatrix}$
Take $B = \begin{pmatrix} \log \mu_1 & 0 \\ 0 & \log \mu_2 \end{pmatrix}$

$$C = PJP^{-1}$$

$$J = \begin{pmatrix} \mu_1 & 0 \\ 0 & \mu_2 \end{pmatrix}$$

or $J = \begin{pmatrix} \mu_1 & 1 \\ 0 & \mu_2 \end{pmatrix}$

also $P^{-1}e^B P = e^{P^{-1}BP}$

Take $\tilde{B} = P^{-1}BP$

$$C = PJP^{-1}$$

$$C = Pe^K P^{-1} = e^{PKP^{-1}}$$

$$B = PKP^{-1} = P \begin{pmatrix} \log \mu_1 & 0 \\ 0 & \log \mu_2 \end{pmatrix} P^{-1}$$

Case 2: $J = \begin{pmatrix} \mu & 1 \\ 0 & \mu \end{pmatrix}$

$$K = \begin{pmatrix} a_1 & a_2 \\ 0 & a_1 \end{pmatrix}$$

$$e^K = \begin{pmatrix} e^{a_1} & a_2 e^{a_1} \\ 0 & e^{a_1} \end{pmatrix}$$

$$K = \begin{pmatrix} \log \mu & 1/\mu \\ 0 & \log \mu \end{pmatrix} \quad \mu \neq 0$$

$$B = PKP^{-1}$$

Jordan Canonical Form

$$J = \begin{bmatrix} J_1 & 0 & & 0 \\ 0 & J_2 & & 0 \\ & & \ddots & \\ 0 & & 0 & J_k \end{bmatrix}$$

where for each i

$$① J_i = [\lambda]$$

$$② J_i = \begin{bmatrix} \lambda_i & 1 & 0 & \dots & 0 \\ 0 & \lambda_i & 1 & \dots & 0 \\ \vdots & \vdots & \vdots & \ddots & \vdots \\ 0 & 0 & 0 & \dots & \lambda_i \end{bmatrix}$$

$$J = \bigoplus_{i=1}^k J_i$$

$$K = \bigoplus_{i=1}^k K_i$$

$$\exp \begin{bmatrix} K_1 & & & \\ & K_2 & & \\ & & \ddots & \\ & & & K_k \end{bmatrix} = \begin{bmatrix} \exp(K_1) & 0 & 0 & 0 \\ 0 & \exp(K_2) & 0 & 0 \\ & & \ddots & \\ 0 & 0 & 0 & \exp(K_k) \end{bmatrix}$$

PROOF OF FLOUQUET'S THEOREM:-

$$\psi'_\omega(t) = \psi'(t+\omega) = A(t+\omega)\psi(t+\omega)$$

$$= A(t)\psi(t+\omega) = A(t)\psi_\omega(t)$$

$\Rightarrow \psi_\omega$ is a soln. matrix

$$\det(\psi_\omega(t)) = \det(\psi(t+\omega)) \neq 0$$

$\Rightarrow \psi(t+\omega)$ is a FSM.

Fix a point $t_0 \in \mathbb{R}$.

$$C_0 = \psi^{-1}(t_0)\psi_\omega(t_0)$$

Note C_0 is a non-singular matrix.

$$\psi_\omega(t_0) = \psi(t_0)C$$

Now observe $\psi(t)C$ is a FSM and agrees with $\psi_\omega(t)$ at t_0 . Hence,

$$\psi_\omega(t) = \psi(t)C$$

$$\psi(t+\omega) = \psi(t)C \quad \forall t \in \mathbb{R}$$

By the existence of \log for $M \in GL_n(\mathbb{R})$

$$\exists B \in M_n(\mathbb{R}) \text{ s.t. } C = \exp(B\omega)$$

Consider $P(t) = \psi(t)\exp(-Bt)$

$$\psi(t) = P(t)\exp(Bt)$$

$$\begin{aligned} P(t+w) &= \psi(t+w) \exp(-B(t+w)) = \psi(t) \exp(-Bt) \exp(-Bw) C \\ &= \psi(t) \exp(-Bt) = P(t) \end{aligned}$$

3/11/2025

Stability of (LHS):-

$$\dot{x}(t) = A(t)x(t)$$

In the 2×2 case, A is a constant matrix.

$$\dot{x}(t) = A(t)x(t)$$

Case 1. A is diagonalizable with eigenvalues α_1 & α_2 .

$$\begin{aligned} x(t) &= ae^{\alpha_1 t} u_1 + be^{\alpha_2 t} u_2 \\ \|x(t)\|^2 &= e^{2\alpha_1 t} \|u_1\|^2 a^2 + e^{2\alpha_2 t} \|u_2\|^2 b^2 \\ &\quad + 2e^{(\alpha_1 + \alpha_2)t} ab \langle u_1, u_2 \rangle \\ &\leq (e^{\alpha_1 t} |a| \|u_1\| + e^{\alpha_2 t} |b| \|u_2\|)^2 < \epsilon \end{aligned}$$

$$e^{\alpha_1 t} |a| \|u_1\| + e^{\alpha_2 t} |b| \|u_2\| < \sqrt{\epsilon}$$

Suppose $\alpha_1, \alpha_2 < 0$,

then $|a| \|u_1\| + |b| \|u_2\| < \sqrt{\epsilon}$

THEOREM: Consider $\dot{x}(t) = A(t)x(t)$ where A is an $n \times n$ real matrix. Then

- Suppose $\exists \lambda$, an eigenvalue of A such that $\text{Re}(\lambda) > 0$ then the trivial soln. is unstable
- Suppose all the eigenvalues with zero real part are simple, and all other eigenvalues have negative real part, then the solution is stable.
- If all eigenvalues of A have negative real part then the solution is asymptotically stable.

Periodic System:-

$$\dot{x}(t) = A(t)x(t)$$

$$A(t+\omega) = A(t)$$

THEOREM: Let u_1, \dots, u_n be the Floquet multipliers of the system. Then the following holds true.

- If $|u_i| < 1 \forall 1 \leq i \leq n$ then the trivial soln. is asymptotically stable.
- Stable if $\forall i, |u_i| \leq 1$
- Unstable if $\exists i, |u_i| > 1$

Kellert & Peterson

Boundary Value Problems:

$$\boxed{\frac{\partial^2 u(t, x)}{\partial x^2} = \frac{1}{c^2} \frac{\partial^2 u(t, x)}{\partial t^2}} \quad \text{One-dim. wave eqn.}$$

$u(t, x) :=$ disp. of the string at x , and time t ,
 $c :=$ propagation speed

$$u(t, 0) = 0, \quad u(t, 1) = 0$$

$$u(0, x) = u(x), \quad \frac{\partial u(0, x)}{\partial t} = v(x)$$

$$u(t, x) = W(t)y(x)$$

$$\frac{1}{c^2} \frac{W''(t)}{W(t)} = \frac{y''(x)}{y(x)} = -\lambda$$

$$\Rightarrow \begin{aligned} y''(x) &= -\lambda y(x) - \textcircled{1} & y(0) &= 0, \quad y(1) = 0 \\ W''(t) &= -c^2 \lambda W(t) - \textcircled{2} \end{aligned}$$

4/11/2025

Stability of Autonomous System

THEOREM: Consider $x'(t) = Ax(t)$. Then the trivial soln.

Stable \Leftrightarrow for any $\lambda \in \sigma(A)$, $\operatorname{Re}(\lambda) \leq 0$ and $m_g(\lambda) = m_a(\lambda) \forall \lambda$ with $\operatorname{Re}(\lambda) = 0$.

Unstable $\Leftrightarrow \exists \lambda \in \sigma(A)$ s.t. $\operatorname{Re}(\lambda) > 0$ or $\exists \lambda \in \sigma(A)$ s.t. $\operatorname{Re}(\lambda) = 0$ & $m_a(\lambda) > m_g(\lambda) \geq 1$

Asymptotic Stable $\Leftrightarrow \operatorname{Re}(\lambda) < 0 \forall \lambda \in \sigma(A)$

Here, $A \in M_n(\mathbb{R})$

$\sigma(A) :=$ the set of all eigenvalues of A
 $\lambda \in \sigma(A)$

$m_g(\lambda) :=$ the geometric multiplicity of λ
 $= \dim(\ker(A - \lambda I))$

$m_a(\lambda) :=$ algebraic multiplicity of λ

Sturm Boundary Value Problems :-

$$\frac{\partial^2 u(t, x)}{\partial x^2} = \frac{1}{c^2} \frac{\partial^2 u(t, x)}{\partial t^2}$$

$$u(t, x) = W(t)y(x)$$

$$\Rightarrow \frac{1}{c^2} \frac{W''(t)}{W(t)} = \frac{y''(x)}{y(x)} = -\lambda \text{ (a constant)}$$

$$\begin{aligned} u(0, x) &= u(x) \\ \frac{\partial u(0, x)}{\partial x} &= v(x) \end{aligned} \quad \text{One-dim.}$$

$$u(t, 0) = 0, \quad u(t, 1) = 0$$

$$\Rightarrow W''(t) + c^2 \lambda W(t) = 0$$

$$\boxed{y''(x) + \lambda y(x) = 0, y(0) = 0, y(1) = 0} \quad \text{--- ①}$$

$$\xi^2 + c^2 \lambda = 0$$

Case ①: $\lambda > 0$

$$\pm i c \sqrt{\lambda} \\ \alpha e^{i c \sqrt{\lambda} t} + \beta e^{-i c \sqrt{\lambda} t}$$

$$W(t) = \alpha \cos c \sqrt{\lambda} t + \beta \sin c \sqrt{\lambda} t$$

$$\xi^2 + \lambda = 0$$

$$y(x) = \gamma \cos \sqrt{\lambda} x + \delta \sin \sqrt{\lambda} x$$

$$y(0) = 0 \Rightarrow \gamma = 0$$

$$y(1) = 0 \\ \delta \sin \sqrt{\lambda} = 0$$

$$\delta = 0 \text{ or } \sin \sqrt{\lambda} = 0$$

$$\Rightarrow \sqrt{\lambda} = n\pi \Rightarrow \lambda = n^2 \pi^2$$

$$\boxed{U_n(t, x) = (\alpha \cos c n \pi t + \beta \sin c n \pi t) \sin n \pi x}$$

DEFINITION (ADJOINT):-

Consider second order ODE,

$$a_0(t) \frac{d^2 x}{dt^2} + a_1(t) \frac{dx}{dt} + a_2(t) x(t) = 0 \quad \text{--- ①}$$

Here: a_0 is twice continuously differentiable & $a_0(t) \neq 0$ on I .
 a_1 is continuously differentiable.
 a_2 is continuous.

The adjoint of ① is the differential equation:

$$\frac{d^2}{dt^2} (a_0(t) x(t)) - \frac{d}{dt} (a_1(t) x(t)) + a_2(t) x(t) = 0$$

$$\Leftrightarrow a_0(t) \frac{d^2 x}{dt^2} + [2a_0'(t) - a_1(t)] \frac{dx}{dt} + (a_0''(t) - a_1'(t) + a_2(t)) x(t) = 0$$

DEFINITION: ① is called **self-adjoint** if ① and its adjoint eqns. are identical. $\Leftrightarrow 2a_0'(t) - a_1(t) = a_1(t)$

$$\Leftrightarrow a_0'(t) = a_1(t)$$

\Leftrightarrow ① can be written in the following form:-

$$\frac{d}{dt} \left(a_0(t) \frac{dx}{dt} \right) + a_2(t) x(t) = 0$$

EXAMPLE: $(1-t^2) \frac{d^2 x}{dt^2} - 2t \frac{dx}{dt} + n(n+1) x(t) = 0$

HOMEWORK:

$$a_0(t) \frac{d^2 x}{dt^2} + a_1(t) \frac{dx}{dt} + a_2(t) x(t) = 0 \quad (*)$$

$$\frac{d}{dt} \left(p(t) \frac{dx}{dt} \right) + Q(t) x(t) = 0 \text{ by multiplying } (*) \text{ by}$$

$$\frac{1}{a_0(t)} \exp \int \frac{a_1(t)}{a_0(t)} dt$$

$$P(t) = \exp \left(\int \frac{a_1(t)}{a_0(t)} dt \right)$$

$$Q(t) = \frac{a_2(t)}{a_0(t)} \exp \left(\int \frac{a_1(t)}{a_0(t)} dt \right)$$

From now on the general, second-order, self-adjoint ordinary DE that we will consider:

$$(p(t)x')' + q(t)x(t) = h(t)$$

6/11/2025

Consider the self-adjoint equation:

$$(p(t)x')' + q(t)x(t) = h(t)$$

Assuming that $p(t)$, $q(t)$, $h(t)$ are continuous on I .

$$\mathcal{D} := \{x \in C(I):$$

DEFINITION: $x(t)$ & $y(t)$ are differentiable fncs, then we define

$$W(x(t), y(t)) = \det \begin{pmatrix} x(t) & y(t) \\ x'(t) & y'(t) \end{pmatrix}$$

Lagrange's Identity: Suppose $x, y \in \mathcal{D}$ then

$$x(t)L(y(t)) - y(t)L(x(t)) = [p(t)W(x(t), y(t))] \quad \forall t \in I$$

Corollary: If x & y are solns of $L(x(t)) \equiv 0$

then $W(x(t), y(t)) = \frac{C}{p(t)}$, where C is a constant $\forall t \in I$.

Sturm-Liouville Boundary Problems: -

$$(p(t)x')' + (\lambda r(t) + q(t))x(t) = 0$$

Together with boundary conditions

$$\alpha x(a) - \beta x'(a) = 0$$

$$\gamma x(b) - \delta x'(b) = 0$$

$$\left. \begin{array}{l} p(t) > 0 \\ I = [a, b] \\ \alpha^2 + \beta^2 > 0 \\ \gamma^2 + \delta^2 > 0 \end{array} \right\} \text{ (SLP)} \quad y(t) \geq 0$$

$$L(x(t)) = (p(t)x')' + q(t)x(t)$$

DEFINITION: $\lambda_0 \in \mathbb{R}$ is called an eigenvalue of (SLP) if $\exists x_0$, a nontrivial funcⁿ s.t.

$$Lx_0(t) = -\lambda_0 x_0(t)$$

satisfying the boundary condition.

(λ_0, x_0) an eigenpair, x_0 is called the eigen function corresponding to λ_0 .

Suppose, given a λ_0 an eigenvalue of (SLP) if any two eigenfuncⁿs corresponding to λ_0 are lin. dependent, then λ_0 is called simple.

EXAMPLE: $x'' = -\lambda x$, $x(0) = 0$, $x(\pi) = 0$

Case I: $\lambda > 0$, $\lambda = \mu^2$

$$x'' + \mu^2 x = 0$$

$$t^2 + \mu^2 = 0$$

$$x(t) = \alpha e^{i\mu t} + \beta e^{-i\mu t}$$

$$= \alpha \cos \mu t + \beta \sin \mu t$$

$$0 = \alpha, 0 = \beta \sin \pi \mu$$

$$\beta \neq 0, \sin \pi \mu = 0 \quad \pi \mu = \pm n\pi$$

$$\mu = \pm n$$

$$\lambda = \mu^2 = n^2$$

$$\lambda = n^2, \quad n_\lambda(t) = \pm \sin nt$$

Case II: $\lambda = 0$.

$$x'' = 0$$

$$x(t) = \alpha + \beta t$$

$$x(0) = 0 \Rightarrow \alpha = 0$$

$$x(\pi) = 0, \beta \pi = 0, \beta = 0$$

Case III: $\lambda = -\mu^2$

$$x'' - \mu^2 x = 0$$

$$x(t) = \alpha e^{\mu t} + \beta e^{-\mu t}$$

$$\begin{pmatrix} 1 & 1 \\ e^{\pi\mu} & e^{-\pi\mu} \end{pmatrix} \begin{pmatrix} \alpha \\ \beta \end{pmatrix} = 0$$

$$x(0) = 0$$

$$\alpha + \beta = 0$$

$$\alpha e^{\pi\mu} + \beta e^{-\pi\mu} = 0$$

DEFINITION: Let $\gamma \in C([a, b], \mathbb{R})$ & assume $\gamma \geq 0$ & not identically equal to zero.

Then on $C([a, b], \mathbb{R})$, we introduce the inner product, defined by

$$\langle x(t), y(t) \rangle_\gamma = \int_a^b x(t)y(t)\gamma(t)dt$$

x & y are orthogonal w.r.t. γ if $\langle x(t), y(t) \rangle_\gamma = 0$

THEOREM: $Lx(t) = -\lambda \gamma(t)x(t)$

$$\alpha x(a) - \beta x'(a) = 0$$

$$\gamma x(b) - \delta x'(b) = 0$$

$$\alpha^2 + \beta^2$$

10/11/2025

THEOREM: Consider the (SLP)

$$(p x')' + (\lambda y(t) + q(t)) x = 0$$

$$\left. \begin{aligned} \alpha x(a) - \beta x'(a) &= 0 \\ \delta x(b) - \gamma x'(b) &= 0 \end{aligned} \right\} \textcircled{BV}$$

When $p > 0$, $\alpha \geq 0$ and $q \in C[a, b]$

The eigenfunctions corresponding to distinct eigen values are orthogonal.
Each eigen value is simple.

PROOF: $(\lambda_1, x_1) \quad (\lambda_2, x_2)$

$$(\lambda_1 - \lambda_2) \langle x_1, x_2 \rangle_y = \left[p(t) W(x_1(t), x_2(t)) \right]_a^b$$

$$W(x_1(t), x_2(t)) \Big|_{t=a} = x_1(a) x_2'(a) - x_2(a) x_1'(a)$$

$$= x_1(a) \frac{\alpha x_2(a)}{\beta} - x_2(a) \frac{\alpha x_1(a)}{\beta} = 0$$

$$\alpha x_j(a) - \beta x_j'(a) = 0$$

$$\beta = 0, W(x_1(t), x_2(t)) \Big|_{t=a} = 0$$

$$(\lambda_1 - \lambda_2) \langle x_1, x_2 \rangle_\delta = 0$$

$$\lambda_1 \neq \lambda_2 \Rightarrow \langle x_1, x_2 \rangle_\delta = 0$$

$$(\lambda_1, x_1), (\lambda_2, x_2)$$

$$(\lambda_1 - \lambda_2) \delta(t) x_1(t) x_2(t) = [p(t) W(x_1, x_2)]$$

$$\Rightarrow p(t) W(x_1, x_2) = C$$

From boundary condiⁿ, $C=0 \Rightarrow W(x_1, x_2)=0$
 $\Rightarrow x_1$ and x_2 are l.d.

STURM-LOUVILLE THEOREM:

Then the (SLP) has an infinite seq. of eigenvalues (λ_n) with $\lambda_n < \lambda_{n+1}$ & $\lim_{n \rightarrow \infty} \lambda_n = \infty$. The eigenfunⁿ corresponding to each λ_n has precisely $(n-1)$ zeros in $[a, b]$.

Oscillation Theory:

Consider

$$(px')' + Q(t)x = 0$$

Prüfer Substitution:

We write

$$px' = r(t) \cos \theta(t)$$

$$x = r(t) \sin \theta(t)$$

$$(px')^2 + x^2 = (r(t))^2$$

$$\tan \theta(t) = \frac{x}{px'}$$

$$\cot \theta(t) = \frac{px'}{x}$$

$$-\operatorname{cosec}^2 \theta(t) \frac{d\theta}{dt} = \frac{(px')'}{x} - \frac{px'^2}{x^2}$$

$$= -Q(t) - \frac{1}{P} \frac{r(t)^2 \cos^2 \theta(t)}{r(t)^2 \sin^2 \theta(t)}$$

$$2r(t)r'(t) = 2px'(px')' + 2xx'$$

$$= 2px'(-Q(t)x(t)) + 2xx'$$

$$= 2r^2(t) \cos \theta(t) - Q(t) \sin \theta(t)$$

$$+ \frac{2r^2(t) \sin \theta(t) \cos \theta(t)}{P}$$

$$\frac{d\theta}{dt} = Q(t) \sin^2 \theta + \frac{1}{P(t)} \cos^2 \theta$$

$$= F(t, \theta) \text{ --- ①}$$

$$\frac{dr}{dt} = \frac{1}{2} r \sin 2\theta \left(\frac{1}{P(t)} - Q(t) \right) \text{ --- ②}$$

PRÜFER
SYSTEM

LEMMA: If (SLP) has non-trivial soln., $\sigma(t)$ never vanishes

Consider the self-adjoint equation

$$(Px')' + Q(t)x(t) = 0 \quad \text{--- (SA)}$$

We say (SA) is oscillatory if it admits a soln. that has more than one zero.

OBSERVATION: If x is a soln. of (SA) on $[a, b]$ and let $t_0 \in [a, b]$ s.t. $x(t_0) = 0$ then $\theta(t_0) = m\pi, m \in \mathbb{Z}$

PROPOSITION: For each $m \in \mathbb{Z}$, \exists at most one point $t_m \in [a, b]$ s.t. $\theta(t_m) = m\pi$.
Moreover if $t < t_m$ then $\theta(t) < m\pi$ and if $t > t_m$, $\theta(t) > m\pi$

PROOF: Consider the constant fncⁿ

$$y(t) = m\pi$$

$$y'(t) = 0 \quad F(t, m\pi) = \frac{1}{P(t)} > 0 = y'(t)$$

Suppose $t_m \in [a, b]$ is such that

$$\theta(t_m) = m\pi = y(t_m)$$

$$\theta(t) > m\pi \quad \forall t > t_m$$

Say, \tilde{t}_m s.t. $\theta(\tilde{t}_m) = m\pi, \tilde{t}_m < t_m \Rightarrow \theta(t_m) > m\pi (*)$

11/11/2025

Consider θ -equations corresponding to two Prüfer systems:

$$\tilde{\theta}' = \tilde{Q} \sin^2 \tilde{\theta} + \frac{1}{\tilde{P}} \cos^2 \tilde{\theta} \quad \tilde{\theta}(a) = \tilde{\theta}_0$$

$$\theta' = Q \sin^2 \theta + \frac{1}{P} \cos^2 \theta = F(t, \theta) \quad \theta(a) = \theta_0$$

PROPOSITION 1: Suppose $Q(t) \geq \tilde{Q}(t) \quad \forall t \in (a, b)$ and $\frac{1}{P(t)} \geq \frac{1}{\tilde{P}(t)} \quad \forall t \in (a, b)$ and assume that $\theta_0 \geq \tilde{\theta}_0$. Then $\theta(t) \geq \tilde{\theta}(t) \quad \forall t \in [a, b]$. Moreover, if $\exists t_* \in (a, b]$ s.t. $\theta(t_*) = \tilde{\theta}(t_*)$ then $\theta(t) = \tilde{\theta}(t) \quad \forall t \in [a, t_*]$

PROOF: $\tilde{\theta}' - F(t, \tilde{\theta}) = \tilde{Q} \sin^2 \tilde{\theta} + \frac{1}{\tilde{P}} \cos^2 \tilde{\theta} - \left(Q \sin^2 \tilde{\theta} + \frac{1}{P} \cos^2 \tilde{\theta} \right)$

$$= \sin^2 \tilde{\theta} (\tilde{Q} - Q) + \cos^2 \tilde{\theta} \left(\frac{1}{\tilde{P}} - \frac{1}{P} \right) \leq 0 = \tilde{\theta}' - F(t, \theta)$$

Since $\tilde{\theta}(a) \leq \theta(a) \Rightarrow \theta(t) \geq \tilde{\theta}(t) \quad \forall t \in [a, b]$

COROLLARY: Suppose in Proposition 1, we have either $Q(t) > \tilde{Q}(t) \quad \forall t \in (a, b)$ or $\frac{1}{P(t)} > \frac{1}{\tilde{P}(t)} \quad \forall t \in (a, b)$. Then $\theta(t) > \tilde{\theta}(t) \quad \forall t \in (a, b)$

PROOF: Suppose $Q(t) > \tilde{Q}(t) \quad \forall t \in (a, b)$. Suppose $\exists t_* \in (a, b]$ s.t. $\theta(t_*) = \tilde{\theta}(t_*)$

$$\theta(t) = \hat{\theta}(t) \quad \forall t \in [a, t_*],$$

$$\underbrace{(Q - \hat{Q})}_{\geq 0} \sin^2 \theta + \underbrace{\left(\frac{1}{p} - \frac{1}{\hat{p}} \right)}_{\geq 0} \cos^2 \theta = 0 \quad \text{on } [a, t_*]$$

$$\Rightarrow \sin^2 \theta(t) = 0, \quad \cos^2 \theta(t) = 1$$

$\Rightarrow \theta$ is constant

$$\theta' = \frac{1}{p}, \quad \theta \text{ is strictly increasing } (*)$$

STURM COMPARISON THEOREM:-

$$\underbrace{\left(\hat{p} \frac{d\hat{x}}{dt} \right)' + \hat{Q}\hat{x} = 0}_{\text{I}} \quad \& \quad \underbrace{\left(p \frac{dx}{dt} \right)' + Qx = 0}_{\text{II}}$$

Suppose $Q(t) \geq \hat{Q}(t)$ & $p(t) \leq \hat{p}(t) \quad \forall t \in [a, b]$. Now, let \hat{x} be a nontrivial soln. of I that has zeros at $c, d \in [a, b]$. Let x be a soln. of II then x has a zero in the interval $[c, d]$. This implies if \hat{x} has n zeros in $[a, b]$ then x has at least $(n-1)$ zeros in the interval $[a, b]$.

$$\hat{x}(c) = 0 = \hat{r}(t) \sin \hat{\theta}(c) \Rightarrow \hat{\theta}(c) = m\pi, m \in \mathbb{Z}.$$

$$\hat{x}(d) = 0 = \hat{r}(t) \cos \hat{\theta}(d) \Rightarrow \hat{\theta}(d) = n\pi, n \in \mathbb{Z}$$

We will assume $\hat{\theta}(c) = 0, \hat{\theta}(d) = n\pi, n \in \mathbb{Z}_+$.

Consider the $\hat{\theta}$ and θ eqns. with initial condiⁿs

$$\hat{\theta}(c) = 0$$

$$\theta(c) \in [0, \pi)$$

Then by Proposition 1, $\theta(t) \geq \hat{\theta}(t) \quad \forall t \in [c, b]$

$$\theta(d) \geq \hat{\theta}(d) = n\pi, \quad n \in \mathbb{Z}^+$$

$$\Rightarrow \exists t \in [c, d] \text{ s.t. } \theta(t) = n\pi$$

$$x(t) = \sin \theta(t) = 0$$

First part